show-int/Simple.v
@@ -16,6 +16,7 @@ Require BinInt.
 Require Coq.Init.Peano.
 Require GHC.Base.
 Require GHC.Char.
+Require GHC.Err.
 Require GHC.Num.
 Require GHC.Real.
 Require GHC.Wf.
@@ -28,14 +29,14 @@ Import GHC.Num.Notations.
 Require Omega.
 Import BinInt.
 
-Lemma showInt_go_termination: forall arg_2__ : GHC.Num.Integer,
-  _GHC.Base.==_ arg_2__ 0%Z = false ->
-  _GHC.Base.<_ arg_2__ 0%Z = false ->
-  BinInt.Z.abs_nat (arg_2__ / 10) < BinInt.Z.abs_nat arg_2__.
+Lemma showInt_go_termination: forall i : GHC.Num.Integer,
+  _GHC.Base.==_ i 0%Z = false ->
+  _GHC.Base.<_ i 0%Z = false ->
+  BinInt.Z.abs_nat (i / 10) < BinInt.Z.abs_nat i.
 Proof.
   intros.
-  assert (0 < arg_2__)%Z. {
-    induction arg_2__; try Omega.omega; Coq.Program.Tactics.program_simpl.
+  assert (0 < i)%Z. {
+    destruct i; try Omega.omega; Coq.Program.Tactics.program_simpl.
     apply Pos2Z.is_pos.
   }
   apply Zabs.Zabs_nat_lt. split.
@@ -55,19 +56,12 @@ Program Definition showInt : GHC.Num.Integer -> GHC.Base.String :=
                 let y := GHC.Real.fromIntegral x in
                 GHC.Char.chr (y GHC.Num.+ GHC.Base.ord (GHC.Char.hs_char__ "0")) in
             let go : GHC.Num.Integer -> GHC.Base.String -> GHC.Base.String :=
-              GHC.Wf.wfFix2 Coq.Init.Peano.lt (fun arg_2__ arg_3__ =>
-                               BinInt.Z.abs_nat arg_2__) _ (fun arg_2__ arg_3__ go =>
-                               match arg_2__, arg_3__ with
-                               | num_4__, s =>
-                                   if Bool.Sumbool.sumbool_of_bool (num_4__ GHC.Base.== #0) then s else
-                                   match arg_2__, arg_3__ with
-                                   | i, s =>
-                                       if Bool.Sumbool.sumbool_of_bool (i GHC.Base.< #0)
-                                       then GHC.Base.hs_string__ ""
-                                       else let 'pair tens ones := GHC.Real.divMod i #10 in
-                                            go tens (cons (digit2char ones) s)
-                                   end
-                               end) in
+              GHC.Wf.wfFix2 Coq.Init.Peano.lt (fun i s => BinInt.Z.abs_nat i) _ (fun i s go =>
+                               if Bool.Sumbool.sumbool_of_bool (i GHC.Base.== #0) then s else
+                               if Bool.Sumbool.sumbool_of_bool (i GHC.Base.< #0)
+                               then GHC.Err.error (GHC.Base.hs_string__ "go {< 0}") else
+                               let 'pair tens ones := GHC.Real.divMod i #10 in
+                               go tens (cons (digit2char ones) s)) in
             match GHC.Base.compare i #0 with
             | Lt => cons (GHC.Char.hs_char__ "-") (go (GHC.Num.negate i) nil)
             | Eq => GHC.Base.hs_string__ "0"
@@ -78,7 +72,7 @@ Solve Obligations with (solve_showInt_termination).
 (* External variables:
      Bool.Sumbool.sumbool_of_bool Eq Gt Lt cons nil pair BinInt.Z.abs_nat
      Coq.Init.Peano.lt GHC.Base.String GHC.Base.compare GHC.Base.op_zeze__
-     GHC.Base.op_zl__ GHC.Base.ord GHC.Char.Char GHC.Char.chr GHC.Num.Integer
-     GHC.Num.fromInteger GHC.Num.negate GHC.Num.op_zp__ GHC.Real.divMod
-     GHC.Real.fromIntegral GHC.Wf.wfFix2
+     GHC.Base.op_zl__ GHC.Base.ord GHC.Char.Char GHC.Char.chr GHC.Err.error
+     GHC.Num.Integer GHC.Num.fromInteger GHC.Num.negate GHC.Num.op_zp__
+     GHC.Real.divMod GHC.Real.fromIntegral GHC.Wf.wfFix2
 *)
