show-int/GhcShow.v
@@ -1,0 +1,201 @@
+(* Default settings (from HsToCoq.Coq.Preamble) *)
+
+Generalizable All Variables.
+
+Unset Implicit Arguments.
+Set Maximal Implicit Insertion.
+Unset Strict Implicit.
+Unset Printing Implicit Defensive.
+
+Require Coq.Program.Tactics.
+Require Coq.Program.Wf.
+
+(* Converted imports: *)
+
+Require BinInt.
+Require Coq.Init.Peano.
+Require GHC.Base.
+Require GHC.Err.
+Require GHC.Num.
+Require GHC.Real.
+Require GHC.Wf.
+Import GHC.Base.Notations.
+Import GHC.Num.Notations.
+
+(* No type declarations to convert. *)
+(* Midamble *)
+
+Require Omega.
+Import BinInt.
+
+Lemma jhead_termination: forall n,
+  _GHC.Base.<_ n 10%Z = false ->
+  Z.abs_nat (n / 10) < Z.abs_nat n.
+Proof.
+  intros.
+  assert (0 < n)%Z. {
+    destruct n; Coq.Program.Tactics.program_simpl.
+    apply Pos2Z.is_pos.
+  }
+  apply Zabs.Zabs_nat_lt. split.
+  - apply Zdiv.Z_div_pos; Omega.omega.
+  - apply Zdiv.Z_div_lt; Omega.omega.
+Qed.
+
+Lemma jblock'_termination: forall d,
+  _GHC.Base.==_ d 1%Z = false ->
+  _GHC.Base.<_ d 1%Z = false ->
+  Z.abs_nat (d - 1) < Z.abs_nat d.
+Proof.
+  intros.
+  assert (0 < d)%Z. {
+    destruct d; Coq.Program.Tactics.program_simpl.
+    apply Pos2Z.is_pos.
+  } apply Zabs.Zabs_nat_lt. Omega.omega.
+Qed.
+
+Lemma jsplitf_termination: forall p n,
+  _GHC.Base.<=_ p 1%Z = false ->
+  _GHC.Base.>_ p n = false ->
+  Z.abs_nat n - Z.abs_nat (p * p - 1) < Z.abs_nat n - Z.abs_nat (p - 1).
+Proof.
+  intros p n Hp1 Hpn.
+  unfold GHC.Base.op_zlze__ in Hp1. unfold GHC.Base.op_zg__ in Hpn. unfold Base.Ord_Integer___ in Hp1,Hpn. simpl in Hp1,Hpn.
+  apply Z.leb_gt in Hp1. apply Z.ltb_ge in Hpn.
+  assert (1 * 1 <= p * p)%Z. {
+    apply Z.mul_le_mono_nonneg; Omega.omega.
+  }
+  rewrite 3! Znat.Zabs2Nat.abs_nat_nonneg by Omega.omega.
+  rewrite <- 2! Znat.Z2Nat.inj_sub by Omega.omega.
+  set (m := (n - (p * p - 1))%Z).
+  destruct (0 <=? m)%Z eqn:Hleb.
+  - apply Z.leb_le in Hleb.
+    rewrite <- 2! Znat.Zabs2Nat.abs_nat_nonneg; try Omega.omega.
+    apply Zabs.Zabs_nat_lt.
+    split. { assumption. }
+    apply Z.sub_le_lt_mono. { apply Z.le_refl. }
+    apply Z.sub_lt_le_mono; try Omega.omega.
+    rewrite <- Z.mul_1_l at 1.
+    apply Z.mul_lt_mono_pos_r; Omega.omega.
+  - apply Z.leb_gt in Hleb.
+    destruct m; inversion Hleb.
+    rewrite Znat.Z2Nat.inj_neg.
+    rewrite <- Znat.Zabs2Nat.abs_nat_nonneg by Omega.omega.
+    rewrite <- Znat.Zabs2Nat.inj_0.
+    apply Zabs.Zabs_nat_lt.
+    Omega.omega.
+Qed.
+
+Ltac solve_integerToString_termination :=
+  Coq.Program.Tactics.program_simpl;
+  first [apply jhead_termination | apply jblock'_termination | apply jsplitf_termination];
+  assumption.
+(* Converted value declarations: *)
+
+Definition quotRemInteger
+   : GHC.Num.Integer ->
+     GHC.Num.Integer -> (GHC.Num.Integer * GHC.Num.Integer)%type :=
+  fun a b => let 'pair q r := GHC.Real.divMod a b in pair q r.
+
+Program Definition integerToString
+           : GHC.Num.Integer -> GHC.Base.String -> GHC.Base.String :=
+          fun n0 cs0 =>
+            let jblock'
+             : GHC.Num.Int -> GHC.Num.Int -> GHC.Base.String -> GHC.Base.String :=
+              GHC.Wf.wfFix3 Coq.Init.Peano.lt (fun d n cs => BinInt.Z.abs_nat d) _ (fun d
+                             n
+                             cs
+                             jblock' =>
+                               let 'pair q r := GHC.Real.divMod n #10 in
+                               if Bool.Sumbool.sumbool_of_bool (d GHC.Base.== #1)
+                               then let 'c := GHC.Base.unsafeChr (GHC.Base.ord (GHC.Char.hs_char__ "0")
+                                                                  GHC.Num.+
+                                                                  n) in
+                                    cons c cs else
+                               if Bool.Sumbool.sumbool_of_bool (d GHC.Base.< #1)
+                               then GHC.Err.errorWithoutStackTrace (GHC.Base.hs_string__ "jblock' {< 1}") else
+                               let 'c := GHC.Base.unsafeChr (GHC.Base.ord (GHC.Char.hs_char__ "0") GHC.Num.+
+                                                             r) in
+                               jblock' (d GHC.Num.- #1) q (cons c cs)) in
+            let jblock := jblock' #18 in
+            let jhead : GHC.Num.Int -> GHC.Base.String -> GHC.Base.String :=
+              GHC.Wf.wfFix2 Coq.Init.Peano.lt (fun n cs => BinInt.Z.abs_nat n) _ (fun n
+                             cs
+                             jhead =>
+                               let 'pair q r := GHC.Real.divMod n #10 in
+                               if Bool.Sumbool.sumbool_of_bool (n GHC.Base.< #10)
+                               then let 'c := GHC.Base.unsafeChr (GHC.Base.ord (GHC.Char.hs_char__ "0")
+                                                                  GHC.Num.+
+                                                                  n) in
+                                    cons c cs else
+                               let 'c := GHC.Base.unsafeChr (GHC.Base.ord (GHC.Char.hs_char__ "0") GHC.Num.+
+                                                             r) in
+                               jhead q (cons c cs)) in
+            let jprintb : list GHC.Num.Integer -> GHC.Base.String -> GHC.Base.String :=
+              fix jprintb arg_20__ arg_21__
+                    := match arg_20__, arg_21__ with
+                       | nil, cs => cs
+                       | cons n ns, cs =>
+                           let 'pair q' r' := quotRemInteger n #1000000000000000000 in
+                           let r := GHC.Num.fromInteger r' in
+                           let q := GHC.Num.fromInteger q' in jblock q (jblock r (jprintb ns cs))
+                       end in
+            let jprinth : list GHC.Num.Integer -> GHC.Base.String -> GHC.Base.String :=
+              fun arg_29__ arg_30__ =>
+                match arg_29__, arg_30__ with
+                | cons n ns, cs =>
+                    let 'pair q' r' := quotRemInteger n #1000000000000000000 in
+                    let r := GHC.Num.fromInteger r' in
+                    let q := GHC.Num.fromInteger q' in
+                    if Bool.Sumbool.sumbool_of_bool (q GHC.Base.> #0)
+                    then jhead q (jblock r (jprintb ns cs))
+                    else jhead r (jprintb ns cs)
+                | nil, _ => GHC.Err.errorWithoutStackTrace (GHC.Base.hs_string__ "jprinth []")
+                end in
+            let jsplitb : GHC.Num.Integer -> list GHC.Num.Integer -> list GHC.Num.Integer :=
+              fix jsplitb arg_39__ arg_40__
+                    := match arg_39__, arg_40__ with
+                       | _, nil => nil
+                       | p, cons n ns =>
+                           let 'pair q r := quotRemInteger n p in
+                           cons q (cons r (jsplitb p ns))
+                       end in
+            let jsplith : GHC.Num.Integer -> list GHC.Num.Integer -> list GHC.Num.Integer :=
+              fun arg_46__ arg_47__ =>
+                match arg_46__, arg_47__ with
+                | p, cons n ns =>
+                    let 'pair q r := quotRemInteger n p in
+                    if Bool.Sumbool.sumbool_of_bool (q GHC.Base.> #0)
+                    then cons q (cons r (jsplitb p ns))
+                    else cons r (jsplitb p ns)
+                | _, nil => GHC.Err.errorWithoutStackTrace (GHC.Base.hs_string__ "jsplith: []")
+                end in
+            let jsplitf : GHC.Num.Integer -> GHC.Num.Integer -> list GHC.Num.Integer :=
+              GHC.Wf.wfFix2 Coq.Init.Peano.lt (fun p n =>
+                               BinInt.Z.abs_nat n - BinInt.Z.abs_nat (p - 1)) _ (fun p n jsplitf =>
+                               if Bool.Sumbool.sumbool_of_bool (p GHC.Base.<= #1)
+                               then GHC.Err.errorWithoutStackTrace (GHC.Base.hs_string__ "jsplitf {<= 1}") else
+                               if Bool.Sumbool.sumbool_of_bool (p GHC.Base.> n) then cons n nil else
+                               jsplith p (jsplitf (p GHC.Num.* p) n)) in
+            let integerToString' : GHC.Num.Integer -> GHC.Base.String -> GHC.Base.String :=
+              fun n cs =>
+                if Bool.Sumbool.sumbool_of_bool (n GHC.Base.< #1000000000000000000)
+                then jhead (GHC.Num.fromInteger n) cs else
+                jprinth (jsplitf (#1000000000000000000 GHC.Num.* #1000000000000000000) n) cs in
+            if Bool.Sumbool.sumbool_of_bool (n0 GHC.Base.< #0)
+            then cons (GHC.Char.hs_char__ "-") (integerToString' (GHC.Num.negate n0)
+                       cs0) else
+            integerToString' n0 cs0.
+Solve Obligations with (solve_integerToString_termination).
+
+Definition showInt : GHC.Num.Integer -> GHC.Base.String :=
+  fun i => integerToString i (GHC.Base.hs_string__ "").
+
+(* External variables:
+     Bool.Sumbool.sumbool_of_bool cons list nil op_zm__ op_zt__ pair BinInt.Z.abs_nat
+     Coq.Init.Peano.lt GHC.Base.String GHC.Base.op_zeze__ GHC.Base.op_zg__
+     GHC.Base.op_zl__ GHC.Base.op_zlze__ GHC.Base.ord GHC.Base.unsafeChr
+     GHC.Err.errorWithoutStackTrace GHC.Num.Int GHC.Num.Integer GHC.Num.fromInteger
+     GHC.Num.negate GHC.Num.op_zm__ GHC.Num.op_zp__ GHC.Num.op_zt__ GHC.Real.divMod
+     GHC.Wf.wfFix2 GHC.Wf.wfFix3
+*)
