show-int/Proofs.v
@@ -1,3 +1,64 @@
-Require Import Prelude.
-Require Import Simple.
-Require Import GhcShow.
+
+Require Coq.Program.Tactics.
+Require Coq.Program.Wf.
+
+Require Prelude.
+Require Simple.
+Require GhcShow.
+Import BinInt.
+
+Example Simple_show_123: Simple.showInt 321%Z = GHC.Base.hs_string__ "321".
+Proof.
+  simpl.
+  unfold Simple.showInt.
+  unfold Wf.wfFix2.
+  unfold Wf.wfFix1.
+  simpl.
+  rewrite ! Coq.Program.Wf.WfExtensionality.fix_sub_eq_ext.
+  simpl.
+  rewrite ! Coq.Program.Wf.WfExtensionality.fix_sub_eq_ext.
+  simpl.
+  rewrite ! Coq.Program.Wf.WfExtensionality.fix_sub_eq_ext.
+  simpl.
+  rewrite ! Coq.Program.Wf.WfExtensionality.fix_sub_eq_ext.
+  simpl.
+  reflexivity.
+Qed.
+
+Example show_321: GhcShow.showInt 321%Z = Simple.showInt 321%Z.
+Proof.
+  unfold Simple.showInt.
+  unfold GhcShow.showInt.
+  unfold GhcShow.integerToString.
+  unfold Wf.wfFix2.
+  unfold Wf.wfFix1.
+  simpl.
+  rewrite ! Coq.Program.Wf.WfExtensionality.fix_sub_eq_ext.
+  simpl.
+  rewrite ! Coq.Program.Wf.WfExtensionality.fix_sub_eq_ext.
+  simpl.
+  rewrite ! Coq.Program.Wf.WfExtensionality.fix_sub_eq_ext.
+  simpl.
+  rewrite ! Coq.Program.Wf.WfExtensionality.fix_sub_eq_ext.
+  simpl.
+  reflexivity.
+Qed.
+
+Example show_n456: GhcShow.showInt (-456)%Z = Simple.showInt (-456)%Z.
+Proof.
+  unfold Simple.showInt.
+  unfold GhcShow.showInt.
+  unfold GhcShow.integerToString.
+  unfold Wf.wfFix2.
+  unfold Wf.wfFix1.
+  simpl.
+  rewrite ! Coq.Program.Wf.WfExtensionality.fix_sub_eq_ext.
+  simpl.
+  rewrite ! Coq.Program.Wf.WfExtensionality.fix_sub_eq_ext.
+  simpl.
+  rewrite ! Coq.Program.Wf.WfExtensionality.fix_sub_eq_ext.
+  simpl.
+  rewrite ! Coq.Program.Wf.WfExtensionality.fix_sub_eq_ext.
+  simpl.
+  reflexivity.
+Qed.
